A first sketch of relational recombination
Trying to understand how the proof resembles the old one and how it
changes, and in particular how relations compose, still without
attempting to prove those -- this will probably be the main quarry.

Intermediate/RecombinationRel.v
@@ -267,11 +267,19 @@ Section Mergeable.
       (* behavior_rel_behavior_all_cids n n'' (FTbc t) (FTbc t'') -> *)
       mem_rel3 mt mt' mt''.
 
+  (* Sketch a simple state relation based on the memory-trace relation, for the
+     sake of expediency. *)
+  Inductive mergeable_states (s s' s'' : CS.state) : Prop :=
+  | mergeable_states_intro : forall t t' t'',
+      mem_rel3 (CS.state_mem s, t) (CS.state_mem s', t') (CS.state_mem s'', t'') ->
+      mergeable_states s s' s''.
+
   (* This "extensional" reading of compatible states depends directly on the
      partial programs concerned (implicitly through the section mechanism) and
      two runs synchronized by their traces. It is a rather strong notion, easy
      to work with and well suited to the purposes of the proof. *)
 
+(*
   Inductive mergeable_states (s s' s'' : CS.state) : Prop :=
     mergeable_states_intro : forall s0 s0' s0'' t t' t'' n n' n'',
       (* Well-formedness conditions. *)
@@ -295,7 +303,6 @@ Section Mergeable.
       behavior_rel_behavior_all_cids n n'' (FTbc t) (FTbc t'') ->
       mergeable_states s s' s''.
 
-(*
   (* RB: NOTE: This induction principle is currently used only in the proofs of
      mergeable_states_pc_same_component and mergeable_states_mergeable_stack. It
      would be interesting to see if (other) proofs benefit from its use, or what
@@ -1333,7 +1340,6 @@ Section MergeSym.
   (* Qed. *)
   Admitted.
 End MergeSym.
-*)
 
 (* Helpers, epsilon and lockstep versions of three-way simulation. *)
 Section ThreewayMultisem1.
@@ -2198,6 +2204,7 @@ Section ThreewayMultisem2.
         simpl in Hcontra. omega.
   Qed.
 End ThreewayMultisem2.
+*)
 
 (* Three-way simulation and its inversion. *)
 Section ThreewayMultisem3.
@@ -2212,154 +2219,157 @@ Section ThreewayMultisem3.
   Let sem'  := CS.sem_non_inform prog'.
   Let sem'' := CS.sem_non_inform prog''.
 
-  Theorem threeway_multisem_star s1 s1'' t s2 s2'' :
-    mergeable_states p c p' c' s1 s1'' ->
-    Star (CS.sem_non_inform (program_link p  c )) s1   t s2   ->
-    Star (CS.sem_non_inform (program_link p' c')) s1'' t s2'' ->
-    Star (CS.sem_non_inform (program_link p  c')) (merge_states ip ic s1 s1'') t (merge_states ip ic s2 s2'').
-    (* /\ mergeable_states ip ic s2 s2'' *)
-  Proof.
-    intros Hmerge1 Hstar12 Hstar12''.
-    inversion Hmerge1 as [_ _ _ Hwfp Hwfc Hwfp' Hwfc' Hmergeable_ifaces Hifacep Hifacec _ _ _ _ _ _].
-    destruct (CS.is_program_component s1 ic) eqn:Hcomp1.
-    - now apply threeway_multisem_star_program.
-    - apply negb_false_iff in Hcomp1.
-      apply (mergeable_states_context_to_program Hmerge1)
-        in Hcomp1.
-      assert (Hmerge2: mergeable_states p c p' c' s2 s2'')
-        by (eapply threeway_multisem_mergeable; eassumption).
-      rewrite program_linkC in Hstar12; try assumption;
-        last now destruct Hmergeable_ifaces.
-      rewrite program_linkC in Hstar12''; try assumption;
-        last now destruct Hmergeable_ifaces; rewrite -Hifacec -Hifacep.
-      rewrite program_linkC; try assumption;
-        last now destruct Hmergeable_ifaces; rewrite -Hifacec.
-      unfold ip, ic.
-      setoid_rewrite merge_states_sym at 1 2; try eassumption.
-      pose proof threeway_multisem_star_program as H.
-      specialize (H c' p' c p).
-      rewrite <- Hifacep, <- Hifacec in H.
-      specialize (H s1'' s1 t s2'' s2).
-      apply H; try assumption.
-      apply mergeable_states_sym in Hmerge1; try assumption;
-        try rewrite -Hifacec; try rewrite -Hifacep; try apply mergeable_interfaces_sym;
-          now auto.
-  Qed.
+  (* Theorem threeway_multisem_star s1 s1'' t s2 s2'' : *)
+  (*   mergeable_states p c p' c' s1 s1'' -> *)
+  (*   Star (CS.sem_non_inform (program_link p  c )) s1   t s2   -> *)
+  (*   Star (CS.sem_non_inform (program_link p' c')) s1'' t s2'' -> *)
+  (*   Star (CS.sem_non_inform (program_link p  c')) (merge_states ip ic s1 s1'') t (merge_states ip ic s2 s2''). *)
+  (*   (* /\ mergeable_states ip ic s2 s2'' *) *)
+  (* Proof. *)
+  (*   intros Hmerge1 Hstar12 Hstar12''. *)
+  (*   inversion Hmerge1 as [_ _ _ Hwfp Hwfc Hwfp' Hwfc' Hmergeable_ifaces Hifacep Hifacec _ _ _ _ _ _]. *)
+  (*   destruct (CS.is_program_component s1 ic) eqn:Hcomp1. *)
+  (*   - now apply threeway_multisem_star_program. *)
+  (*   - apply negb_false_iff in Hcomp1. *)
+  (*     apply (mergeable_states_context_to_program Hmerge1) *)
+  (*       in Hcomp1. *)
+  (*     assert (Hmerge2: mergeable_states p c p' c' s2 s2'') *)
+  (*       by (eapply threeway_multisem_mergeable; eassumption). *)
+  (*     rewrite program_linkC in Hstar12; try assumption; *)
+  (*       last now destruct Hmergeable_ifaces. *)
+  (*     rewrite program_linkC in Hstar12''; try assumption; *)
+  (*       last now destruct Hmergeable_ifaces; rewrite -Hifacec -Hifacep. *)
+  (*     rewrite program_linkC; try assumption; *)
+  (*       last now destruct Hmergeable_ifaces; rewrite -Hifacec. *)
+  (*     unfold ip, ic. *)
+  (*     setoid_rewrite merge_states_sym at 1 2; try eassumption. *)
+  (*     pose proof threeway_multisem_star_program as H. *)
+  (*     specialize (H c' p' c p). *)
+  (*     rewrite <- Hifacep, <- Hifacec in H. *)
+  (*     specialize (H s1'' s1 t s2'' s2). *)
+  (*     apply H; try assumption. *)
+  (*     apply mergeable_states_sym in Hmerge1; try assumption; *)
+  (*       try rewrite -Hifacec; try rewrite -Hifacep; try apply mergeable_interfaces_sym; *)
+  (*         now auto. *)
+  (* Qed. *)
   (* JT: TODO: improve this proof *)
 
-  Corollary star_simulation s1 s1'' t s2 s2'' :
-    mergeable_states p c p' c' s1 s1'' ->
-    Star sem   s1   t s2   ->
-    Star sem'' s1'' t s2'' ->
-    Star sem'  (merge_states ip ic s1 s1'') t (merge_states ip ic s2 s2'') /\
-    mergeable_states p c p' c' s2 s2''.
-  Proof.
-    intros. split.
-    - now apply threeway_multisem_star.
-    - eapply threeway_multisem_mergeable; eassumption.
-  Qed.
+  Corollary star_simulation sigma sigma_inv s1 s1' s1'' t t'' s2 s2'' :
+    mergeable_states p sigma sigma_inv s1 s1' s1'' ->
+    Star sem   s1   t   s2   ->
+    Star sem'' s1'' t'' s2'' ->
+    mem_rel2 p sigma sigma_inv (CS.state_mem s2, t) (CS.state_mem s2'', t'') ->
+  exists t' s2',
+    Star sem'  s1' t' s2' /\
+    mergeable_states p sigma sigma_inv s2 s2' s2''.
+  Admitted.
+  (* Proof. *)
+  (*   intros. split. *)
+  (*   - now apply threeway_multisem_star. *)
+  (*   - eapply threeway_multisem_mergeable; eassumption. *)
+  (* Qed. *)
 
   (* [DynShare]
      The following tactic applies program_store_from_partialized_memory
      and program_alloc_from_partialized_memory, which will both fail.
    *)
-  Ltac t_threeway_multisem_step_inv_program gps1 gps1'' Hmerge Hnotin Hifacec:=
-    match goal with
-    (* Memory operations. *)
-    | Hstore : Memory.store _ _ _ = _ |- _ =>
-      apply program_store_from_partialized_memory in Hstore as [mem1_ Hstore];
-        try eassumption
-    | Halloc : Memory.alloc _ _ _ = _ |- _ =>
-      apply program_alloc_from_partialized_memory in Halloc as [mem1_ [ptr_ Halloc]];
-        try assumption
-    (* Calls. *)
-    | Hget : EntryPoint.get _ _ _ = _ |- _ =>
-      apply (genv_entrypoints_interface_some) with (p' := prog) in Hget as [b' Hget];
-      last (simpl; congruence);
-      try assumption
-    (* Returns. *)
-    | Hcons : ?PC' :: ?GPS' = ?GPS (* merge_states_stack *) |- _ =>
-      destruct GPS as [| frame1' gps1'] eqn:Hgps; [discriminate |];
-      destruct gps1 as [| frame1 gps1]; [now destruct gps1'' |];
-      destruct gps1'' as [| frame1'' gps1'']; [easy |];
-      inversion Hcons; subst PC' GPS';
-      assert (Heq : Pointer.component frame1 = Pointer.component frame1')
-        by (unfold merge_states_stack in Hgps;
-            inversion Hgps as [[Hframe Hdummy]];
-            unfold merge_frames;
-            destruct (Pointer.component frame1 \in domm ip) eqn:Hcase; rewrite Hcase;
-            [ reflexivity
-            | eapply mergeable_states_cons_domm; last exact Hmerge; eassumption]);
-      rewrite <- Heq
-    | _ => idtac
-    end;
-    [eexists;
-    CS.step_of_executing];
-      try eassumption; try congruence; try reflexivity;
-      try (simpl; rewrite Hifacec; eassumption);
-      match goal with
-      (* Memory operations. *)
-      | Hload : Memory.load _ _ = _ |- Memory.load _ _ = _ =>
-        unfold merge_states_mem in Hload;
-        erewrite <- program_load_to_partialized_memory_strong in Hload;
-        try exact Hmerge; eassumption
-      (* Jumps. *)
-      | Hlabel : find_label_in_component _ _ _ = _ |- find_label_in_component _ _ _ = _ =>
-        rewrite find_label_in_component_program_link_left;
-        rewrite find_label_in_component_program_link_left in Hlabel;
-        try eassumption; simpl in *; congruence
-      | Hlabel : find_label_in_procedure _ _ _ = _ |- find_label_in_procedure _ _ _ = _ =>
-        rewrite find_label_in_procedure_program_link_left;
-        rewrite find_label_in_procedure_program_link_left in Hlabel;
-        try eassumption; simpl in *; congruence
-      (* Calls. *)
-      | Himp : imported_procedure _ _ _ _ |- imported_procedure _ _ _ _ =>
-        rewrite imported_procedure_unionm_left; [| assumption];
-        rewrite Hifacec in Hnotin; now rewrite imported_procedure_unionm_left in Himp
-      | _ => idtac
-      end;
-    [apply execution_invariant_to_linking with (c1 := c')];
-    try congruence;
-    try eassumption.
-      (* try eassumption; [congruence]. *)
+  (* Ltac t_threeway_multisem_step_inv_program gps1 gps1'' Hmerge Hnotin Hifacec:= *)
+  (*   match goal with *)
+  (*   (* Memory operations. *) *)
+  (*   | Hstore : Memory.store _ _ _ = _ |- _ => *)
+  (*     apply program_store_from_partialized_memory in Hstore as [mem1_ Hstore]; *)
+  (*       try eassumption *)
+  (*   | Halloc : Memory.alloc _ _ _ = _ |- _ => *)
+  (*     apply program_alloc_from_partialized_memory in Halloc as [mem1_ [ptr_ Halloc]]; *)
+  (*       try assumption *)
+  (*   (* Calls. *) *)
+  (*   | Hget : EntryPoint.get _ _ _ = _ |- _ => *)
+  (*     apply (genv_entrypoints_interface_some) with (p' := prog) in Hget as [b' Hget]; *)
+  (*     last (simpl; congruence); *)
+  (*     try assumption *)
+  (*   (* Returns. *) *)
+  (*   | Hcons : ?PC' :: ?GPS' = ?GPS (* merge_states_stack *) |- _ => *)
+  (*     destruct GPS as [| frame1' gps1'] eqn:Hgps; [discriminate |]; *)
+  (*     destruct gps1 as [| frame1 gps1]; [now destruct gps1'' |]; *)
+  (*     destruct gps1'' as [| frame1'' gps1'']; [easy |]; *)
+  (*     inversion Hcons; subst PC' GPS'; *)
+  (*     assert (Heq : Pointer.component frame1 = Pointer.component frame1') *)
+  (*       by (unfold merge_states_stack in Hgps; *)
+  (*           inversion Hgps as [[Hframe Hdummy]]; *)
+  (*           unfold merge_frames; *)
+  (*           destruct (Pointer.component frame1 \in domm ip) eqn:Hcase; rewrite Hcase; *)
+  (*           [ reflexivity *)
+  (*           | eapply mergeable_states_cons_domm; last exact Hmerge; eassumption]); *)
+  (*     rewrite <- Heq *)
+  (*   | _ => idtac *)
+  (*   end; *)
+  (*   [eexists; *)
+  (*   CS.step_of_executing]; *)
+  (*     try eassumption; try congruence; try reflexivity; *)
+  (*     try (simpl; rewrite Hifacec; eassumption); *)
+  (*     match goal with *)
+  (*     (* Memory operations. *) *)
+  (*     | Hload : Memory.load _ _ = _ |- Memory.load _ _ = _ => *)
+  (*       unfold merge_states_mem in Hload; *)
+  (*       erewrite <- program_load_to_partialized_memory_strong in Hload; *)
+  (*       try exact Hmerge; eassumption *)
+  (*     (* Jumps. *) *)
+  (*     | Hlabel : find_label_in_component _ _ _ = _ |- find_label_in_component _ _ _ = _ => *)
+  (*       rewrite find_label_in_component_program_link_left; *)
+  (*       rewrite find_label_in_component_program_link_left in Hlabel; *)
+  (*       try eassumption; simpl in *; congruence *)
+  (*     | Hlabel : find_label_in_procedure _ _ _ = _ |- find_label_in_procedure _ _ _ = _ => *)
+  (*       rewrite find_label_in_procedure_program_link_left; *)
+  (*       rewrite find_label_in_procedure_program_link_left in Hlabel; *)
+  (*       try eassumption; simpl in *; congruence *)
+  (*     (* Calls. *) *)
+  (*     | Himp : imported_procedure _ _ _ _ |- imported_procedure _ _ _ _ => *)
+  (*       rewrite imported_procedure_unionm_left; [| assumption]; *)
+  (*       rewrite Hifacec in Hnotin; now rewrite imported_procedure_unionm_left in Himp *)
+  (*     | _ => idtac *)
+  (*     end; *)
+  (*   [apply execution_invariant_to_linking with (c1 := c')]; *)
+  (*   try congruence; *)
+  (*   try eassumption. *)
+  (*     (* try eassumption; [congruence]. *) *)
 
-  Theorem threeway_multisem_step_inv_program s1 s1'' t s2' :
-    CS.is_program_component s1 ic ->
-    mergeable_states p c p' c' s1 s1'' ->
-    Step sem' (merge_states ip ic s1 s1'') t s2' ->
-  exists s2,
-    Step sem                      s1       t s2.
-  Proof.
-    intros Hpc Hmerge Hstep.
-    inversion Hmerge as [_ _ _ Hwfp Hwfc Hwfp' Hwfc' Hmergeable_ifaces Hifacep Hifacec _ _ _ _ _ _].
-    destruct s1 as [[[[gps1 mem1] regs1] pc1] addrs1].
-    destruct s1'' as [[[[gps1'' mem1''] regs1''] pc1''] addrs1''].
-    inversion Hmergeable_ifaces as [Hlinkable _].
-    pose proof linkable_implies_linkable_mains Hwfp Hwfc Hlinkable as Hmain_linkability.
-    assert (Hlinkable' := Hlinkable); rewrite Hifacep Hifacec in Hlinkable'.
-    pose proof linkable_implies_linkable_mains Hwfp' Hwfc' Hlinkable' as Hmain_linkability'.
-    pose proof is_program_component_pc_in_domm Hpc Hmerge as Hdomm.
-    pose proof is_program_component_pc_in_domm Hpc Hmerge as Hdomm'.
-    pose proof CS.is_program_component_pc_notin_domm _ _ Hpc as Hnotin; unfold ic in Hnotin;
-    assert (Hmains : linkable_mains p c')
-      by (apply linkable_implies_linkable_mains; congruence).
-    rewrite (mergeable_states_merge_program _ Hmerge) in Hstep;
-      try assumption.
-    pose proof linking_well_formedness Hwfp Hwfc Hlinkable as Hwfprog.
-    pose proof linking_well_formedness Hwfp' Hwfc' Hlinkable' as Hwfprog'.
-    assert (Hlinkable'' := Hlinkable); rewrite Hifacec in Hlinkable''.
-    pose proof linking_well_formedness Hwfp Hwfc' Hlinkable'' as Hwfprog''.
+  (* Theorem threeway_multisem_step_inv_program s1 s1'' t s2' : *)
+  (*   CS.is_program_component s1 ic -> *)
+  (*   mergeable_states p c p' c' s1 s1'' -> *)
+  (*   Step sem' (merge_states ip ic s1 s1'') t s2' -> *)
+  (* exists s2, *)
+  (*   Step sem                      s1       t s2. *)
+  (* Proof. *)
+  (*   intros Hpc Hmerge Hstep. *)
+  (*   inversion Hmerge as [_ _ _ Hwfp Hwfc Hwfp' Hwfc' Hmergeable_ifaces Hifacep Hifacec _ _ _ _ _ _]. *)
+  (*   destruct s1 as [[[[gps1 mem1] regs1] pc1] addrs1]. *)
+  (*   destruct s1'' as [[[[gps1'' mem1''] regs1''] pc1''] addrs1'']. *)
+  (*   inversion Hmergeable_ifaces as [Hlinkable _]. *)
+  (*   pose proof linkable_implies_linkable_mains Hwfp Hwfc Hlinkable as Hmain_linkability. *)
+  (*   assert (Hlinkable' := Hlinkable); rewrite Hifacep Hifacec in Hlinkable'. *)
+  (*   pose proof linkable_implies_linkable_mains Hwfp' Hwfc' Hlinkable' as Hmain_linkability'. *)
+  (*   pose proof is_program_component_pc_in_domm Hpc Hmerge as Hdomm. *)
+  (*   pose proof is_program_component_pc_in_domm Hpc Hmerge as Hdomm'. *)
+  (*   pose proof CS.is_program_component_pc_notin_domm _ _ Hpc as Hnotin; unfold ic in Hnotin; *)
+  (*   assert (Hmains : linkable_mains p c') *)
+  (*     by (apply linkable_implies_linkable_mains; congruence). *)
+  (*   rewrite (mergeable_states_merge_program _ Hmerge) in Hstep; *)
+  (*     try assumption. *)
+  (*   pose proof linking_well_formedness Hwfp Hwfc Hlinkable as Hwfprog. *)
+  (*   pose proof linking_well_formedness Hwfp' Hwfc' Hlinkable' as Hwfprog'. *)
+  (*   assert (Hlinkable'' := Hlinkable); rewrite Hifacec in Hlinkable''. *)
+  (*   pose proof linking_well_formedness Hwfp Hwfc' Hlinkable'' as Hwfprog''. *)
 
-    (* [DynShare]
-       Fails because of the program_store_from_partialized_memory and
-       program_alloc_from_partialized_memory
-     *)
-    (*
-    inversion Hstep; subst;
-      t_threeway_multisem_step_inv_program gps1 gps1'' Hmerge Hnotin Hifacec.
-  Qed.
-     *)
-  Admitted.
+  (*   (* [DynShare] *)
+  (*      Fails because of the program_store_from_partialized_memory and *)
+  (*      program_alloc_from_partialized_memory *)
+  (*    *) *)
+  (*   (* *)
+  (*   inversion Hstep; subst; *)
+  (*     t_threeway_multisem_step_inv_program gps1 gps1'' Hmerge Hnotin Hifacec. *)
+  (* Qed. *)
+  (*    *) *)
+  (* Admitted. *)
 End ThreewayMultisem3.
 
 (* Theorems on initial states for main simulation. *)
@@ -2389,61 +2399,69 @@ Section ThreewayMultisem4.
   Let sem'  := CS.sem_non_inform prog'.
   Let sem'' := CS.sem_non_inform prog''.
 
-  Lemma initial_states_mergeability s s'' :
-    initial_state sem   s   ->
-    initial_state sem'' s'' ->
-    mergeable_states p c p' c' s s''.
-  Proof.
-    simpl. unfold CS.initial_state.
-    intros Hini Hini''.
-    apply mergeable_states_intro with (s0 := s) (s0'' := s'') (t := E0); subst;
-      try assumption;
-      reflexivity || now apply star_refl.
-  Qed.
+  (* Lemma initial_states_mergeability s s'' : *)
+  (*   initial_state sem   s   -> *)
+  (*   initial_state sem'' s'' -> *)
+  (*   mergeable_states p c p' c' s s''. *)
+  (* Proof. *)
+  (*   simpl. unfold CS.initial_state. *)
+  (*   intros Hini Hini''. *)
+  (*   apply mergeable_states_intro with (s0 := s) (s0'' := s'') (t := E0); subst; *)
+  (*     try assumption; *)
+  (*     reflexivity || now apply star_refl. *)
+  (* Qed. *)
+
+  Variables sigma sigma_inv : addr_t -> addr_t.
 
   Lemma match_initial_states s s'' :
     initial_state sem   s   ->
     initial_state sem'' s'' ->
-    initial_state sem'  (merge_states ip ic s s'') /\
-    mergeable_states p c p' c' s s''.
+  exists s',
+    initial_state sem'  s'  /\
+    mergeable_states p sigma sigma_inv s s' s''.
   Proof.
     intros Hini Hini''.
-    inversion Hmergeable_ifaces as [Hlinkable _].
-    pose proof initial_states_mergeability Hini Hini'' as Hmerge.
-    pose proof linkable_implies_linkable_mains Hwfp Hwfc Hlinkable as Hmain_linkability.
-    simpl in *. unfold CS.initial_state in *. subst.
-    split; last assumption.
-    (* Expose structure of initial states. *)
-    rewrite !CS.initial_machine_state_after_linking; try congruence;
-      last (apply interface_preserves_closedness_r with (p2 := c); try assumption;
-            now apply interface_implies_matching_mains).
-    unfold merge_states, merge_memories, merge_registers, merge_pcs; simpl.
-    (* Memory simplifictions. *)
-    rewrite (prepare_procedures_memory_left Hlinkable).
-    unfold ip. erewrite Hifacep at 1. rewrite Hifacep Hifacec in Hlinkable.
-    rewrite (prepare_procedures_memory_right Hlinkable).
-    (* Case analysis on main and related simplifications. *)
-    destruct (Component.main \in domm ip) eqn:Hcase;
-      rewrite Hcase.
-    - pose proof domm_partition_notin_r _ _ Hmergeable_ifaces _ Hcase as Hnotin.
-      rewrite (CS.prog_main_block_no_main _ Hwfc Hnotin).
-      rewrite Hifacec in Hnotin. now rewrite (CS.prog_main_block_no_main _ Hwfc' Hnotin).
-    - (* Symmetric case. *)
-      assert (Hcase' : Component.main \in domm ic).
-      { pose proof domm_partition_program_link_in_neither Hwfp Hwfc Hprog_is_closed as H.
-        rewrite Hcase in H.
-        destruct (Component.main \in domm ic) eqn:Hcase''.
-        - reflexivity.
-        - rewrite Hcase'' in H.
-          exfalso; now apply H.
-      }
-      pose proof domm_partition_notin _ _ Hmergeable_ifaces _ Hcase' as Hnotin.
-      rewrite (CS.prog_main_block_no_main _ Hwfp Hnotin).
-      rewrite Hifacep in Hnotin. now rewrite (CS.prog_main_block_no_main _ Hwfp' Hnotin).
-  Qed.
+    eexists. split.
+    - unfold initial_state, CS.initial_machine_state. reflexivity.
+    - admit.
+  Admitted.
+  (*   inversion Hmergeable_ifaces as [Hlinkable _]. *)
+  (*   pose proof initial_states_mergeability Hini Hini'' as Hmerge. *)
+  (*   pose proof linkable_implies_linkable_mains Hwfp Hwfc Hlinkable as Hmain_linkability. *)
+  (*   simpl in *. unfold CS.initial_state in *. subst. *)
+  (*   split; last assumption. *)
+  (*   (* Expose structure of initial states. *) *)
+  (*   rewrite !CS.initial_machine_state_after_linking; try congruence; *)
+  (*     last (apply interface_preserves_closedness_r with (p2 := c); try assumption; *)
+  (*           now apply interface_implies_matching_mains). *)
+  (*   unfold merge_states, merge_memories, merge_registers, merge_pcs; simpl. *)
+  (*   (* Memory simplifictions. *) *)
+  (*   rewrite (prepare_procedures_memory_left Hlinkable). *)
+  (*   unfold ip. erewrite Hifacep at 1. rewrite Hifacep Hifacec in Hlinkable. *)
+  (*   rewrite (prepare_procedures_memory_right Hlinkable). *)
+  (*   (* Case analysis on main and related simplifications. *) *)
+  (*   destruct (Component.main \in domm ip) eqn:Hcase; *)
+  (*     rewrite Hcase. *)
+  (*   - pose proof domm_partition_notin_r _ _ Hmergeable_ifaces _ Hcase as Hnotin. *)
+  (*     rewrite (CS.prog_main_block_no_main _ Hwfc Hnotin). *)
+  (*     rewrite Hifacec in Hnotin. now rewrite (CS.prog_main_block_no_main _ Hwfc' Hnotin). *)
+  (*   - (* Symmetric case. *) *)
+  (*     assert (Hcase' : Component.main \in domm ic). *)
+  (*     { pose proof domm_partition_program_link_in_neither Hwfp Hwfc Hprog_is_closed as H. *)
+  (*       rewrite Hcase in H. *)
+  (*       destruct (Component.main \in domm ic) eqn:Hcase''. *)
+  (*       - reflexivity. *)
+  (*       - rewrite Hcase'' in H. *)
+  (*         exfalso; now apply H. *)
+  (*     } *)
+  (*     pose proof domm_partition_notin _ _ Hmergeable_ifaces _ Hcase' as Hnotin. *)
+  (*     rewrite (CS.prog_main_block_no_main _ Hwfp Hnotin). *)
+  (*     rewrite Hifacep in Hnotin. now rewrite (CS.prog_main_block_no_main _ Hwfp' Hnotin). *)
+  (* Qed. *)
 End ThreewayMultisem4.
 
 (* Remaining theorems for main simulation.  *)
+(*
 Section ThreewayMultisem5.
   Variables p c p' c' : program.
 
@@ -2562,6 +2580,7 @@ Section ThreewayMultisem5.
       contradiction.
   Qed.
 End ThreewayMultisem5.
+*)
 
 (* Main simulation theorem. *)
 Section Recombination.
@@ -2596,66 +2615,65 @@ Section Recombination.
      This result is currently doing the legwork of going from a simulation on
      stars to one on program behaviors without direct mediation from the CompCert
      framework. *)
-  Theorem recombination_prefix m :
-    does_prefix sem   m ->
-    does_prefix sem'' m ->
-    does_prefix sem'  m.
-  Proof.
-    unfold does_prefix.
-    intros [b [Hbeh Hprefix]] [b'' [Hbeh'' Hprefix'']].
-    assert (Hst_beh := Hbeh). assert (Hst_beh'' := Hbeh'').
-    apply CS.program_behaves_inv_non_inform in Hst_beh   as [s1   [Hini1   Hst_beh  ]].
-    apply CS.program_behaves_inv_non_inform in Hst_beh'' as [s1'' [Hini1'' Hst_beh'']].
-    destruct m as [tm | tm | tm].
-    - destruct b   as [t   | ? | ? | ?]; try contradiction.
-      destruct b'' as [t'' | ? | ? | ?]; try contradiction.
-      simpl in Hprefix, Hprefix''. subst t t''.
-      inversion Hst_beh   as [? s2   Hstar12   Hfinal2   | | |]; subst.
-      inversion Hst_beh'' as [? s2'' Hstar12'' Hfinal2'' | | |]; subst.
-      exists (Terminates tm). split; last reflexivity.
-      pose proof match_initial_states Hwfp Hwfc Hwfp' Hwfc' Hmergeable_ifaces Hifacep Hifacec
-           Hprog_is_closed Hprog_is_closed' Hini1 Hini1'' as [Hini1' Hmerge1].
-      pose proof star_simulation Hmerge1 Hstar12 Hstar12'' as [Hstar12' Hmerge2].
-      apply program_runs with (s := merge_states ip ic s1 s1'');
-        first assumption.
-      apply state_terminates with (s' := merge_states ip ic s2 s2'');
-        first assumption.
-      now apply match_final_states with (p' := p').
-    - destruct b   as [? | ? | ? | t  ]; try contradiction.
-      destruct b'' as [? | ? | ? | t'']; try contradiction.
-      simpl in Hprefix, Hprefix''. subst t t''.
-      inversion Hst_beh   as [| | | ? s2   Hstar12   Hstep2   Hfinal2  ]; subst.
-      inversion Hst_beh'' as [| | | ? s2'' Hstar12'' Hstep2'' Hfinal2'']; subst.
-      exists (Goes_wrong tm). split; last reflexivity.
-      pose proof match_initial_states Hwfp Hwfc Hwfp' Hwfc' Hmergeable_ifaces Hifacep Hifacec
-           Hprog_is_closed Hprog_is_closed' Hini1 Hini1'' as [Hini' Hmerge1].
-      pose proof star_simulation Hmerge1 Hstar12 Hstar12'' as [Hstar12' Hmerge2].
-      apply program_runs with (s := merge_states ip ic s1 s1'');
-        first assumption.
-      apply state_goes_wrong with (s' := merge_states ip ic s2 s2'');
-        first assumption.
-      + eapply match_nostep; eassumption.
-      + eapply match_nofinal; eassumption.
-    - (* Here we talk about the stars associated to the behaviors, without
-         worrying now about connecting them to the existing initial states. *)
-      destruct (CS.behavior_prefix_star_non_inform Hbeh Hprefix)
-        as [s1_ [s2 [Hini1_ Hstar12]]].
-      destruct (CS.behavior_prefix_star_non_inform Hbeh'' Hprefix'')
-        as [s1''_ [s2'' [Hini1''_ Hstar12'']]].
-      pose proof match_initial_states Hwfp Hwfc Hwfp' Hwfc' Hmergeable_ifaces Hifacep Hifacec
-           Hprog_is_closed Hprog_is_closed' Hini1_ Hini1''_ as [Hini1' Hmerge1].
-      pose proof star_simulation Hmerge1 Hstar12 Hstar12'' as [Hstar12' Hmerge2].
-      eapply program_behaves_finpref_exists;
-        last now apply Hstar12'.
-      assumption.
-  Qed.
+  (* Theorem recombination_prefix m : *)
+  (*   does_prefix sem   m -> *)
+  (*   does_prefix sem'' m -> *)
+  (*   does_prefix sem'  m. *)
+  (* Proof. *)
+  (*   unfold does_prefix. *)
+  (*   intros [b [Hbeh Hprefix]] [b'' [Hbeh'' Hprefix'']]. *)
+  (*   assert (Hst_beh := Hbeh). assert (Hst_beh'' := Hbeh''). *)
+  (*   apply CS.program_behaves_inv_non_inform in Hst_beh   as [s1   [Hini1   Hst_beh  ]]. *)
+  (*   apply CS.program_behaves_inv_non_inform in Hst_beh'' as [s1'' [Hini1'' Hst_beh'']]. *)
+  (*   destruct m as [tm | tm | tm]. *)
+  (*   - destruct b   as [t   | ? | ? | ?]; try contradiction. *)
+  (*     destruct b'' as [t'' | ? | ? | ?]; try contradiction. *)
+  (*     simpl in Hprefix, Hprefix''. subst t t''. *)
+  (*     inversion Hst_beh   as [? s2   Hstar12   Hfinal2   | | |]; subst. *)
+  (*     inversion Hst_beh'' as [? s2'' Hstar12'' Hfinal2'' | | |]; subst. *)
+  (*     exists (Terminates tm). split; last reflexivity. *)
+  (*     pose proof match_initial_states Hwfp Hwfc Hwfp' Hwfc' Hmergeable_ifaces Hifacep Hifacec *)
+  (*          Hprog_is_closed Hprog_is_closed' Hini1 Hini1'' as [Hini1' Hmerge1]. *)
+  (*     pose proof star_simulation Hmerge1 Hstar12 Hstar12'' as [Hstar12' Hmerge2]. *)
+  (*     apply program_runs with (s := merge_states ip ic s1 s1''); *)
+  (*       first assumption. *)
+  (*     apply state_terminates with (s' := merge_states ip ic s2 s2''); *)
+  (*       first assumption. *)
+  (*     now apply match_final_states with (p' := p'). *)
+  (*   - destruct b   as [? | ? | ? | t  ]; try contradiction. *)
+  (*     destruct b'' as [? | ? | ? | t'']; try contradiction. *)
+  (*     simpl in Hprefix, Hprefix''. subst t t''. *)
+  (*     inversion Hst_beh   as [| | | ? s2   Hstar12   Hstep2   Hfinal2  ]; subst. *)
+  (*     inversion Hst_beh'' as [| | | ? s2'' Hstar12'' Hstep2'' Hfinal2'']; subst. *)
+  (*     exists (Goes_wrong tm). split; last reflexivity. *)
+  (*     pose proof match_initial_states Hwfp Hwfc Hwfp' Hwfc' Hmergeable_ifaces Hifacep Hifacec *)
+  (*          Hprog_is_closed Hprog_is_closed' Hini1 Hini1'' as [Hini' Hmerge1]. *)
+  (*     pose proof star_simulation Hmerge1 Hstar12 Hstar12'' as [Hstar12' Hmerge2]. *)
+  (*     apply program_runs with (s := merge_states ip ic s1 s1''); *)
+  (*       first assumption. *)
+  (*     apply state_goes_wrong with (s' := merge_states ip ic s2 s2''); *)
+  (*       first assumption. *)
+  (*     + eapply match_nostep; eassumption. *)
+  (*     + eapply match_nofinal; eassumption. *)
+  (*   - (* Here we talk about the stars associated to the behaviors, without *)
+  (*        worrying now about connecting them to the existing initial states. *) *)
+  (*     destruct (CS.behavior_prefix_star_non_inform Hbeh Hprefix) *)
+  (*       as [s1_ [s2 [Hini1_ Hstar12]]]. *)
+  (*     destruct (CS.behavior_prefix_star_non_inform Hbeh'' Hprefix'') *)
+  (*       as [s1''_ [s2'' [Hini1''_ Hstar12'']]]. *)
+  (*     pose proof match_initial_states Hwfp Hwfc Hwfp' Hwfc' Hmergeable_ifaces Hifacep Hifacec *)
+  (*          Hprog_is_closed Hprog_is_closed' Hini1_ Hini1''_ as [Hini1' Hmerge1]. *)
+  (*     pose proof star_simulation Hmerge1 Hstar12 Hstar12'' as [Hstar12' Hmerge2]. *)
+  (*     eapply program_behaves_finpref_exists; *)
+  (*       last now apply Hstar12'. *)
+  (*     assumption. *)
+  (* Qed. *)
 
   (* RB: NOTE: [DynShare] This definition may be used to expose a simpler
      relation, which would still fit the theorem statement, though one of the
      explicit connections would be lost. *)
   (* Definition prefix_rel m m' := *)
   (*   exists n n', behavior_rel_behavior_all_cids n n' m m'. *)
-
   Theorem recombination_prefix_rel m m'' n n'' :
     does_prefix sem   m ->
     does_prefix sem'' m'' ->
@@ -2663,6 +2681,59 @@ Section Recombination.
   exists m' n',
     does_prefix sem'  m' /\
     behavior_rel_behavior_all_cids n' n   m' m.
+  Proof.
+    (* unfold does_prefix. *)
+    intros [b [Hbeh Hprefix]] [b'' [Hbeh'' Hprefix'']] Hrel.
+    (* Invert prefix executions to expose their initial states (and full program
+       behaviors. *)
+    assert (Hst_beh := Hbeh). assert (Hst_beh'' := Hbeh'').
+    apply CS.program_behaves_inv_non_inform in Hst_beh   as [s1   [Hini1   Hst_beh  ]].
+    apply CS.program_behaves_inv_non_inform in Hst_beh'' as [s1'' [Hini1'' Hst_beh'']].
+    (* Suppose we can establish the relation between the initial states of the
+       two runs and the initial state of the recombined program. *)
+    pose (s1' := CS.initial_machine_state (program_link p c')).
+    assert
+      (exists sigma sigma_inv, mergeable_states p sigma sigma_inv s1 s1' s1'')
+      as [sigma [sigma_inv Hmerge1]]
+      by admit.
+    (* In the standard proof, because the two executions produce the same
+       prefix, we know that the two runs either terminate, go wrong or are
+       unfinished. The third case is probably the most interesting here. *)
+    destruct (CS.behavior_prefix_star_non_inform Hbeh Hprefix)
+      as [s1_ [s2 [Hini1_ Hstar12]]].
+    destruct (CS.behavior_prefix_star_non_inform Hbeh'' Hprefix'')
+      as [s1''_ [s2'' [Hini1''_ Hstar12'']]].
+    pose proof match_initial_states Hwfp Hwfc Hwfp' Hwfc' Hmergeable_ifaces Hifacep Hifacec
+         Hprog_is_closed Hprog_is_closed' sigma sigma_inv Hini1_ Hini1''_
+      as [s1'_ [Hini1' Hmerge1_]].
+    (* By determinacy of initial program states: *)
+    assert (Heq1 : s1 = s1_) by admit.
+    assert (Heq1' : s1' = s1'_) by admit.
+    assert (Heq1'' : s1'' = s1''_) by admit.
+    subst s1_ s1'_ s1''_.
+    clear Hini1_ Hini1''_ Hmerge1_.
+    (* Now we should be able to apply a modified star simulation. *)
+    pose proof star_simulation Hmerge1 Hstar12 Hstar12'' as [t' [s2' [Hstar12' Hmerge2]]].
+    {
+      (* For this, however, we need to be able to establish the memory
+         relation between the two, in principle starting from [Hmerge1] and
+         [Hrel]. *)
+      admit.
+    }
+    (* Actually, we need to ensure that the executed trace corresponds to a
+       finite prefix behavior (and that the obtained relation extends to
+       it.) *)
+    assert (exists m', t' = finpref_trace m') as [m' Heq] by admit; subst.
+    (* Now we can instantiate the quantifiers (assume the mapping [n'] can be
+       obtained easily). *)
+    exists m'. eexists. split.
+    - (* In principle, the same lemma that was used for the third case of the
+         original proof should work here. *)
+      pose proof program_behaves_finpref_exists Hini1' Hstar12'
+             as [beh' [Hbeh' Hprefix']].
+      exists beh'. admit.
+    - (* We would then be left to establish the trace relation. *)
+      admit.
   Admitted.
 
 End Recombination.
